# Note about "Yet Another Haskell Tutorial"
Tags: Haskell

------

# Exercises Solutions

 

http://en.wikibooks.org/wiki/Haskell/YAHT

 

# Exercise 3.10

 

Save the following scripts in SumInputs.hs:

 

 module Main where 
 main = do 
  inputNumbers <- getNumber 
  putStrLn ("The sum is " ++ show (sum inputNumbers)) 
  putStrLn ("The product is " ++ show (foldr (*) 1 inputNumbers)) 
  printFactorials inputNumbers 
 getNumber = do 
  putStrLn "Give me a number (or 0 to stop): " 
  number <- getLine 
  let num = read number 
  if num == 0 
   then return [] 
   else do 
    rest <- getNumber 
    return (num : rest) 
 printFactorials [] = putStrLn "" 
 printFactorials (x:xs) = do 
  putStrLn (show x ++ " factorial is: " ++ show (factorial x)) 
  printFactorials xs 
 factorial 1 = 1 
 factorial n = n * factorial (n-1) 

 

* Run it in ghci: main

* Compile and run in console:

 

 ghc --make SumInputs.hs -o myfac

 ./myfac

 

 

# Exercise 4.4 & 4.5

 

 data Pair a b = Pair a b 
 pairFst (Pair x y) = x 
 pairSnd (Pair x y) = y 
 data Triple a b c = Triple a b c 
 tripleFst :: Triple a b c -> a 
 tripleFst (Triple a b c) = a 
 tripleSnd (Triple a b c) = b 
 tripleThr (Triple a b c) = c 
 data Quadruple a b = Quadruple a a b b deriving (Show) 
 firstTwo :: Quadruple a b -> [a] 
 -- you can't write it as: ... -> [a, a]. This is not a valid type expression? 
 firstTwo (Quadruple w x y z) = [w, x]

 lastTwo :: Quadruple a b -> [b] 
 lastTwo (Quadruple w x y z) = [y, z] 

 

# Exercise 4.6

 

 data Tuple a b c d = Tuple1 a 
      | Tuple2 a b 
      | Tuple3 a b c 
      | Tuple4 a b c d 
      deriving (Show) 
 tuple1 :: Tuple a b c d -> a 
 tuple1 (Tuple1 x) = x 
 tuple1 (Tuple2 x y) = x 
 tuple1 (Tuple3 x y z) = x 
 tuple1 (Tuple4 x y z t) = x 
 tuple2 :: Tuple a b c d -> Maybe b 
 tuple2 (Tuple1 x) = Nothing 
 tuple2 (Tuple2 x y) = Just y 
 tuple2 (Tuple3 x y z) = Just y 
 tuple2 (Tuple4 x y z t) = Just y 
 tuple3 :: Tuple a b c d -> Maybe c 
 tuple3 (Tuple1 x) = Nothing 
 tuple3 (Tuple2 x y) = Nothing 
 tuple3 (Tuple3 x y z) = Just z 
 tuple3 (Tuple4 x y z t) = Just z 
 tuple4 :: Tuple a b c d -> Maybe d 
 tuple4 (Tuple1 x) = Nothing 
 tuple4 (Tuple2 x y) = Nothing 
 tuple4 (Tuple3 x y z) = Nothing 
 tuple4 (Tuple4 x y z t) = Just t 

 

Pattern matching plays a big role in tuple-like data structure.